Proved (memAtomicWoQInl <= memAtomicWoQ);
(plugged it into the main proof)

examples/MemAtomic.v
@@ -1,7 +1,7 @@
 Require Import Bool String List.
-Require Import Lib.CommonTactics Lib.ilist Lib.Word Lib.Indexer.
+Require Import Lib.CommonTactics Lib.FMap Lib.Struct Lib.Reflection Lib.ilist Lib.Word Lib.Indexer.
 Require Import Kami.Syntax Kami.Notations Kami.Semantics Kami.Specialize Kami.Duplicate Kami.RefinementFacts.
-Require Import Kami.Wf Kami.ParametricSyntax Kami.ParametricEquiv Kami.Tactics.
+Require Import Kami.SemFacts Kami.Wf Kami.ParametricSyntax Kami.ParametricEquiv Kami.Tactics.
 Require Import Ex.MemTypes Ex.SC Ex.Fifo.
 
 Set Implicit Arguments.
@@ -42,26 +42,33 @@ Section Middleman.
     Hypothesis HinName: index 0 indexSymbol (inName -- "deq") = None.
     Hypothesis HoutName: index 0 indexSymbol (outName -- "enq") = None.
 
+    Definition getReqI (i: nat) := MethodSig (inName -- "deq" __ i)() : Struct RqFromProc.
+    Definition setRepI (i: nat) := MethodSig (outName -- "enq" __ i)(Struct RsToProc) : Void.
+
+    Definition processLdInlGen: GenAction Void Void :=
+      fun ty =>
+        (Calli req <- { getReq | HinName } ();
+           Assert !#req!RqFromProc@."op";
+           Read memv <- "mem";
+           LET ldval <- #memv@[#req!RqFromProc@."addr"];
+           LET rep <- STRUCT { "data" ::= #ldval } :: Struct RsToProc;
+           Calli { setRep | HoutName } (#rep);
+           Retv)%kami_gen.
+
+    Definition processStInlGen: GenAction Void Void :=
+      fun ty =>
+        (Calli req <- { getReq | HinName } ();
+           Assert #req!RqFromProc@."op";
+           Read memv <- "mem";
+           Write "mem" <- #memv@[ #req!RqFromProc@."addr" <- #req!RqFromProc@."data" ];
+           LET rep <- STRUCT { "data" ::= $$Default } :: Struct RsToProc;
+           Calli { setRep | HoutName } (#rep);
+           Retv)%kami_gen.
+
     Definition memAtomicWoQInlM := META {
       Register "mem" : Vector (Data lgDataBytes) addrSize <- Default
-
-      with Repeat Rule till n by "processLd" :=
-        Calli req <- { getReq | HinName } ();
-        Assert !#req!RqFromProc@."op";
-        Read memv <- "mem";
-        LET ldval <- #memv@[#req!RqFromProc@."addr"];
-        LET rep <- STRUCT { "data" ::= #ldval } :: Struct RsToProc;
-        Calli { setRep | HoutName } (#rep);
-        Retv
-
-      with Repeat Rule till n by "processSt" :=
-        Calli req <- { getReq | HinName } ();
-        Assert #req!RqFromProc@."op";
-        Read memv <- "mem";
-        Write "mem" <- #memv@[ #req!RqFromProc@."addr" <- #req!RqFromProc@."data" ];
-        LET rep <- STRUCT { "data" ::= $$Default } :: Struct RsToProc;
-        Calli { setRep | HoutName } (#rep);
-        Retv
+      with Repeat Rule till n by "processLd" := (processLdInlGen _)
+      with Repeat Rule till n by "processSt" := (processStInlGen _)
     }.
     
   End MemAtomicWoQInl.
@@ -69,7 +76,9 @@ Section Middleman.
 End Middleman.
 
 Hint Unfold mid memAtomicWoQInlM : ModuleDefs.
-Hint Unfold RqFromProc RsToProc getReq setRep exec processLd processSt : MethDefs.
+Hint Unfold RqFromProc RsToProc getReq setRep exec
+     getReqI setRepI processLdInlGen processStInlGen
+     processLd processSt : MethDefs.
 
 Section MemAtomic.
   Variables (addrSize fifoSize lgDataBytes: nat).
@@ -176,8 +185,6 @@ Section MemAtomicWoQ.
 
 End MemAtomicWoQ.
 
-Require Import Lib.FMap Lib.Reflection.
-
 Section MemAtomicWoQInl.
   Variables addrSize lgDataBytes: nat.
   Variable n: nat.
@@ -185,27 +192,269 @@ Section MemAtomicWoQInl.
   Definition memAtomicWoQ_regMap (r: RegsT) := r.
   Definition memAtomicWoQ_ruleMap (o: RegsT) (rn: string) := Some rn.
 
+  Lemma memAtomicWoQInl_refines_memAtomicWoQ_ld:
+    forall o u cs i
+           (H: (i <= n)%nat)
+           (HAction:
+              SemAction
+                o (getActionFromGen string_of_nat natToVoid
+                                    (processLdInlGen "rqFromProc" "rsToProc"
+                                                     addrSize lgDataBytes eq_refl eq_refl) i
+                                    type) u cs WO),
+      Step (memAtomicWoQ addrSize lgDataBytes n) o u
+           {| annot := Some (Some ("processLd") __ (i)); defs := []%fmap; calls := cs |}.
+  Proof.
+    intros; apply step_consistent.
+    invertActionRep; clear H0 H3 H4.
+
+    evar (execLabel: {x : SignatureT & SignT x}).
+    match goal with
+    | [ |- StepInd _ _ _ {| annot := ?ann; defs := _; calls := ?cs |} ] =>
+      assert ({| annot := ann; defs := []%fmap; calls := cs |}
+              = hide {| annot := ann;
+                        defs := ["exec" __ i <- execLabel]%fmap;
+                        calls := cs +["exec" __ i <- execLabel]%fmap |}) as Hl
+          by (unfold hide; simpl; f_equal; meq)
+    end.
+    rewrite Hl; constructor.
+
+    - clear Hl.
+      eapply SubstepsCons.
+      + eapply SubstepsCons.
+        * apply SubstepsNil.
+        * (* processLd *)
+          eapply SingleRule.
+          { instantiate
+              (1:= fun ty =>
+                     Renaming.renameAction
+                       (specializer (midQ addrSize lgDataBytes) i)
+                       (@processLd "rqFromProc" "rsToProc" addrSize lgDataBytes ty)).
+            instantiate (1:= "processLd"%string __ i).
+
+            replace (getRules (memAtomicWoQ addrSize lgDataBytes n))
+            with (getRules (mids addrSize lgDataBytes n))
+              by (simpl; rewrite app_nil_r; reflexivity).
+            apply getRules_duplicate_in; auto.
+            simpl; tauto.
+          }
+          { kinv_constr.
+            instantiate (1:= x); simpl.
+            rewrite H2; reflexivity.
+          }
+        * repeat split; auto.
+        * reflexivity.
+        * reflexivity.
+      + (* exec *)
+        eapply SingleMeth.
+        * instantiate
+            (1:= {| attrName := "exec"%string __ i;
+                    attrType :=
+                      (getMethFromGen
+                         string_of_nat
+                         natToVoid
+                         (existT _ {| arg := Struct (RqFromProc addrSize lgDataBytes);
+                                      ret := Struct (RsToProc lgDataBytes) |}
+                                 (@memInstExec addrSize lgDataBytes))
+                         i) |}).
+
+          replace (getDefsBodies (memAtomicWoQ addrSize lgDataBytes n))
+          with (getDefsBodies (minst addrSize lgDataBytes n))
+            by (simpl; unfold mids; rewrite getDefsBodies_duplicate_nil by reflexivity;
+                rewrite app_nil_l; reflexivity).
+          simpl; rewrite app_nil_r.
+          apply repMeth_in.
+          apply getNatListToN_le; auto.
+        * kinv_constr; auto; try eassumption.
+          instantiate (1:= x); simpl.
+          rewrite H2; reflexivity.
+        * reflexivity.
+      + repeat split; auto.
+        simpl; findeq.
+      + reflexivity.
+      + repeat (rewrite specializer_dom;
+                [|apply specializable_disj_dom_img; reflexivity|cbn; tauto]).
+        unfold mergeLabel, getLabel; f_equal.
+        * unfold execLabel; meq.
+        * meq.
+
+    - rewrite <-Hl; clear Hl; split.
+      + apply M.KeysDisj_empty.
+      + simpl; unfold memAtomicWoQ.
+        rewrite getDefs_app.
+        unfold mids; rewrite getDefs_duplicate_nil by reflexivity.
+        rewrite app_nil_l.
+
+        match goal with
+        | [ |- M.KeysDisj (M.add _ _ (M.add _ ?v _)) _ ] =>
+          remember v as val eqn:Heqv; clear
+        end.
+        induction n.
+        * cbn; unfold M.KeysDisj; intros.
+          findeq; try (inv H; [discriminate|inv H0]).
+        * cbn; rewrite app_nil_r; unfold M.KeysDisj; intros.
+          inv H.
+          { findeq; try (inv H; [discriminate|inv H0]). }
+          { apply IHn0; cbn; rewrite app_nil_r; auto. }
+  Qed.
+
+  Lemma memAtomicWoQInl_refines_memAtomicWoQ_st:
+    forall o u cs i
+           (H: (i <= n)%nat)
+           (HAction:
+              SemAction
+                o (getActionFromGen string_of_nat natToVoid
+                                    (processStInlGen "rqFromProc" "rsToProc"
+                                                     addrSize lgDataBytes eq_refl eq_refl) i
+                                    type) u cs WO),
+      Step (memAtomicWoQ addrSize lgDataBytes n) o u
+           {| annot := Some (Some ("processSt") __ (i)); defs := []%fmap; calls := cs |}.
+  Proof.
+    intros; apply step_consistent.
+    invertActionRep; clear H0 H4 H5.
+
+    evar (execLabel: {x : SignatureT & SignT x}).
+    match goal with
+    | [ |- StepInd _ _ _ {| annot := ?ann; defs := _; calls := ?cs |} ] =>
+      assert ({| annot := ann; defs := []%fmap; calls := cs |}
+              = hide {| annot := ann;
+                        defs := ["exec" __ i <- execLabel]%fmap;
+                        calls := cs +["exec" __ i <- execLabel]%fmap |}) as Hl
+          by (unfold hide; simpl; f_equal; meq)
+    end.
+    rewrite Hl; constructor.
+
+    - clear Hl.
+      eapply SubstepsCons.
+      + eapply SubstepsCons.
+        * apply SubstepsNil.
+        * (* processSt *)
+          eapply SingleRule.
+          { instantiate
+              (1:= fun ty =>
+                     Renaming.renameAction
+                       (specializer (midQ addrSize lgDataBytes) i)
+                       (@processSt "rqFromProc" "rsToProc" addrSize lgDataBytes ty)).
+            instantiate (1:= "processSt"%string __ i).
+
+            replace (getRules (memAtomicWoQ addrSize lgDataBytes n))
+            with (getRules (mids addrSize lgDataBytes n))
+              by (simpl; rewrite app_nil_r; reflexivity).
+            apply getRules_duplicate_in; auto.
+            simpl; tauto.
+          }
+          { kinv_constr.
+            instantiate (1:= x); simpl; auto.
+          }
+        * repeat split; auto.
+        * reflexivity.
+        * reflexivity.
+      + (* exec *)
+        eapply SingleMeth.
+        * instantiate
+            (1:= {| attrName := "exec"%string __ i;
+                    attrType :=
+                      (getMethFromGen
+                         string_of_nat
+                         natToVoid
+                         (existT _ {| arg := Struct (RqFromProc addrSize lgDataBytes);
+                                      ret := Struct (RsToProc lgDataBytes) |}
+                                 (@memInstExec addrSize lgDataBytes))
+                         i) |}).
+
+          replace (getDefsBodies (memAtomicWoQ addrSize lgDataBytes n))
+          with (getDefsBodies (minst addrSize lgDataBytes n))
+            by (simpl; unfold mids; rewrite getDefsBodies_duplicate_nil by reflexivity;
+                rewrite app_nil_l; reflexivity).
+          simpl; rewrite app_nil_r.
+          apply repMeth_in.
+          apply getNatListToN_le; auto.
+        * eapply SemIfElseFalse; kinv_constr; auto; try eassumption.
+          instantiate (1:= x); simpl.
+          rewrite H2; reflexivity.
+        * reflexivity.
+      + repeat split; auto.
+        simpl; findeq.
+      + reflexivity.
+      + repeat (rewrite specializer_dom;
+                [|apply specializable_disj_dom_img; reflexivity|cbn; tauto]).
+        unfold mergeLabel, getLabel; f_equal.
+        * unfold execLabel; meq.
+        * meq.
+
+    - rewrite <-Hl; clear Hl; split.
+      + apply M.KeysDisj_empty.
+      + simpl; unfold memAtomicWoQ.
+        rewrite getDefs_app.
+        unfold mids; rewrite getDefs_duplicate_nil by reflexivity.
+        rewrite app_nil_l.
+
+        match goal with
+        | [ |- M.KeysDisj (M.add _ _ (M.add _ ?v _)) _ ] =>
+          remember v as val eqn:Heqv; clear
+        end.
+        induction n.
+        * cbn; unfold M.KeysDisj; intros.
+          findeq; try (inv H; [discriminate|inv H0]).
+        * cbn; rewrite app_nil_r; unfold M.KeysDisj; intros.
+          inv H.
+          { findeq; try (inv H; [discriminate|inv H0]). }
+          { apply IHn0; cbn; rewrite app_nil_r; auto. }
+  Qed.
+
   Lemma memAtomicWoQInl_refines_memAtomicWoQ:
     memAtomicWoQInl addrSize lgDataBytes n <<== memAtomicWoQ addrSize lgDataBytes n.
   Proof.
-    apply stepRefinement with (ruleMap:= memAtomicWoQ_ruleMap) (theta:= memAtomicWoQ_regMap);
-      [admit|].
+    apply stepRefinement with (ruleMap:= memAtomicWoQ_ruleMap) (theta:= memAtomicWoQ_regMap).
 
-    intros; clear H.
-    apply SemFacts.step_zero in H0; [|reflexivity]; dest.
-    destruct l as [ann ds cs]; simpl in *; subst; cbn.
-    destruct ann as [r|].
+    - unfold memAtomicWoQ_regMap.
+      f_equal; simpl.
+      unfold mids; rewrite getRegInits_duplicate_nil by reflexivity.
+      rewrite app_nil_l; reflexivity.
 
-    - inv H0.
-      + exists (M.empty _); cbn; split; auto.
-        admit. (* empty-step *)
+    - intros; clear H.
+      apply step_zero in H0; [|reflexivity]; dest.
+      destruct l as [ann ds cs]; simpl in *; subst; cbn.
+      destruct ann as [r|];
+        [|inv H0; exists (M.empty _); cbn; split; auto; apply step_empty; auto].
+      inv H0; [exists (M.empty _); cbn; split; auto; apply step_empty; auto|].
+      rewrite idElementwiseId.
+      unfold Datatypes.id, memAtomicWoQ_regMap, memAtomicWoQ_ruleMap.
+      
+      exists u; split; auto.
 
-      + unfold memAtomicWoQ_ruleMap.
-        admit.
-
-    - inv H0; exists (M.empty _); cbn; split; auto.
-      admit. (* empty-step *)
-  Admitted.
-
+      assert (exists i,
+                 le i n /\
+                 (k = "processLd"%string __ i /\
+                  a = getActionFromGen
+                        string_of_nat
+                        natToVoid
+                        (processLdInlGen "rqFromProc" "rsToProc" addrSize lgDataBytes
+                                         eq_refl eq_refl) i \/
+                  k = "processSt"%string __ i /\
+                  a = getActionFromGen
+                        string_of_nat
+                        natToVoid
+                        (processStInlGen "rqFromProc" "rsToProc" addrSize lgDataBytes
+                                         eq_refl eq_refl) i)) as Ha.
+      { clear -HInRules; cbn in HInRules.
+        rewrite app_nil_r in HInRules.
+        apply in_app_or in HInRules; destruct HInRules.
+        { apply repRule_in_exists in H; destruct H as [i ?]; dest; subst.
+          exists i; split.
+          { apply getNatListToN_le; auto. }
+          { left; repeat split. }
+        }
+        { apply repRule_in_exists in H; destruct H as [i ?]; dest; subst.
+          exists i; split.
+          { apply getNatListToN_le; auto. }
+          { right; repeat split. }
+        }
+      }
+      clear HInRules; destruct Ha as [i ?]; dest.
+      destruct H0; dest; subst.
+      + apply memAtomicWoQInl_refines_memAtomicWoQ_ld; auto.
+      + apply memAtomicWoQInl_refines_memAtomicWoQ_st; auto.
+  Qed.
+    
 End MemAtomicWoQInl.
-  
+
